WIP Resync dot_lty with unary_lr

theories/Dot/misc_unused/dot_lty.v
@@ -1,11 +1,17 @@
 From iris.proofmode Require Import tactics.
-From D Require Import iris_prelude lty.
+From D Require Export iris_prelude.
+From D Require Import ty_interp_subst_lemmas lty.
 From D.Dot Require Import syn syn.path_repl dlang_inst path_wp lr_syn_aux.
 From D.pure_program_logic Require Import lifting.
 
 Notation "'λI' x .. y , t" := (fun x => .. (fun y => t%I) ..)
   (at level 200, x binder, y binder, right associativity, only parsing,
   format "'[  ' '[  ' 'λI'  x  ..  y ']' ,  '/' t ']'") : function_scope.
+
+Include TyInterpLemmas VlSorts dlang_inst.
+
+(** Override notation from [dlang] to specify scope. *)
+Notation "⟦ T ⟧" := (ty_interp T%ty).
 
 Implicit Types (Σ : gFunctors).
 Implicit Types
@@ -26,30 +32,32 @@ Global Arguments dlty_car {_} !_ _ _ /.
 Global Arguments dlty_label {_} _ /.
 Global Existing Instance dlty_persistent.
 
+Local Notation IntoPersistent' P := (IntoPersistent false P P).
 
-(* Definition sdtp `{!dlangG Σ} Γ l (φ : dlty Σ) d : iProp Σ :=
-  □∀ ρ, ⌜path_includes (pv (ids 0)) ρ [(l, d)] ⌝ → s⟦Γ⟧* ρ → lift_dlty φ l ρ d.|[ρ]. *)
-
-Definition sdtp `{!dlangG Σ} Γ l (φ : dlty Σ) d : iProp Σ :=
-  (⌜ l = dlty_label φ ⌝ ∧
-    □∀ ρ, s⟦Γ⟧* ρ → dlty_car φ ρ d.|[ρ])%I.
-Global Arguments sdtp /.
-Notation "Γ s⊨ { l := d  } : T" := (sdtp Γ l T d) (at level 64, d, l, T at next level).
-
-Definition sptp `{!dlangG Σ} Γ (τ : olty Σ 0) p i: iProp Σ :=
-  □∀ ρ, s⟦Γ⟧* ρ -∗
-    ▷^i path_wp (p.|[ρ]) (λ v, oClose τ ρ v).
-
-Notation "Γ s⊨p p : τ , i" := (sptp Γ τ p i) (at level 74, p, τ, i at next level).
-
-(*
-  Even if semantic types use infinite substitutions, we can still reuse the
-  current stamping theory, based on finite substitutions.
-*)
-Section Sec.
+Section Defs.
   Context `{HdotG: dlangG Σ} {i : nat}.
   Implicit Types (φ : hoEnvD Σ i) (τ : olty Σ i).
+  Implicit Types (T : olty Σ 0) (TD : dlty Σ).
 
+  Definition lift_dlty (φ : dlty Σ) l : envPred dm Σ :=
+    λI ρ d, ⌜ dlty_label φ = l ⌝ ∧ dlty_car φ ρ d.
+
+  (* Definition sdtp Γ l (φ : dlty Σ) d : iProp Σ :=
+    □∀ ρ, ⌜path_includes (pv (ids 0)) ρ [(l, d)] ⌝ → s⟦Γ⟧* ρ → lift_dlty φ l ρ d.|[ρ]. *)
+
+  Definition sdtp Γ TD l d : iProp Σ :=
+    (⌜ l = dlty_label TD ⌝ ∧
+      □∀ ρ, s⟦Γ⟧* ρ → dlty_car TD ρ d.|[ρ])%I.
+  Global Arguments sdtp /.
+
+  Definition sptp Γ T p i: iProp Σ :=
+    □∀ ρ, s⟦Γ⟧* ρ -∗
+      ▷^i path_wp (p.|[ρ]) (λ v, oClose T ρ v).
+
+  (*
+    Even if semantic types use infinite substitutions, we can still reuse the
+    current stamping theory, based on finite substitutions.
+  *)
   Definition leadsto_envD_equiv s σ (φ : hoEnvD Σ i) : iProp Σ :=
     (∃ (φ' : hoEnvD Σ i),
       ⌜φ ≡ (λ args ρ, φ' args (∞ σ.|[ρ]))⌝ ∧ s ↝n[ i ] φ')%I.
@@ -57,13 +65,16 @@ Section Sec.
 
   Definition dm_to_type d i (ψ : hoD Σ i) : iProp Σ :=
     (∃ s σ, ⌜ d = dtysem σ s ⌝ ∧ s ↗n[ σ , i ] ψ)%I.
-End Sec.
+End Defs.
 
+Notation "Γ s⊨ { l := d  } : T" := (sdtp Γ T l d) (at level 64, d, l, T at next level).
+Notation "Γ s⊨p p : τ , i" := (sptp Γ τ p i) (at level 74, p, τ, i at next level).
 Notation "s ↝[  σ  ] φ" := (leadsto_envD_equiv s σ φ) (at level 20).
 Notation "d ↗n[ i  ] ψ" := (dm_to_type d i ψ) (at level 20).
 
 Section dm_to_type.
   Context `{HdotG: dlangG Σ}.
+
   Global Instance dm_to_type_persistent d i ψ: Persistent (d ↗n[ i ] ψ) := _.
 
   Lemma dm_to_type_agree d i ψ1 ψ2 args v : d ↗n[ i ] ψ1 -∗ d ↗n[ i ] ψ2 -∗ ▷ (ψ1 args v ≡ ψ2 args v).
@@ -94,44 +105,178 @@ Section SemTypes.
    (* (ψ : vl -d> iPropO Σ) (φ : envD Σ)  *)
 
   Program Definition lift_dinterp_vl (T : dlty Σ): olty Σ 0 :=
-    olty0 (λ ρ v, (∃ d, ⌜v @ dlty_label T ↘ d⌝ ∧ dlty_car T ρ d)%I).
+    olty0 (λI ρ v, (∃ d, ⌜v @ dlty_label T ↘ d⌝ ∧ dlty_car T ρ d)).
 
   (* Rewrite using (higher) semantic kinds! *)
   Definition oDTMem l τ1 τ2 : dlty Σ := Dlty l
-    (λ ρ d,
+    (λI ρ d,
     ∃ ψ, (d ↗n[ 0 ] ψ) ∧
        □ ((∀ v, ▷ τ1 vnil ρ v → ▷ □ ψ vnil v) ∧
-          (∀ v, ▷ □ ψ vnil v → ▷ τ2 vnil ρ v)))%I.
+          (∀ v, ▷ □ ψ vnil v → ▷ τ2 vnil ρ v))).
 
   Definition oTTMem l τ1 τ2 :=
     lift_dinterp_vl (oDTMem l τ1 τ2).
 
   Definition oDVMem l τ : dlty Σ := Dlty l
-    (λ ρ d, ∃ pmem, ⌜d = dpt pmem⌝ ∧ path_wp pmem (oClose τ ρ))%I.
+    (λI ρ d, ∃ pmem, ⌜d = dpt pmem⌝ ∧ path_wp pmem (oClose τ ρ)).
 
   Definition oTVMem l τ :=
     lift_dinterp_vl (oDVMem l τ).
-(*
-  Program Definition oInterp T := Olty ⟦ T ⟧ _.
-  Next Obligation. rewrite /vclosed=>*. by rewrite interp_vclosed. Qed. *)
 
   Definition oTSel p (l : label) :=
-    olty0 (λ ρ v, path_wp p.|[ρ]
-      (λ vp, ∃ ψ d, ⌜vp @ l ↘ d⌝ ∧ d ↗n[ 0 ] ψ ∧ ▷ □ ψ vnil v))%I.
+    olty0 (λI ρ v, path_wp p.|[ρ]
+      (λ vp, ∃ ψ d, ⌜vp @ l ↘ d⌝ ∧ d ↗n[ 0 ] ψ ∧ ▷ □ ψ vnil v)).
 
+  Lemma oTSel_pv w (l : label) args ρ v :
+    oTSel (pv w) l args ρ v ⊣⊢
+      ∃ ψ d, ⌜w.[ρ] @ l ↘ d⌝ ∧ d ↗n[ 0 ] ψ ∧ ▷ □ ψ vnil v.
+  Proof. by rewrite /= path_wp_pv. Qed.
+
+  Definition oPSing p : olty Σ 0 :=
+    olty0 (λI ρ v, ⌜alias_paths p.|[ρ] (pv v)⌝).
+
+  (* Paolo: This definition is contractive (similarly to what's useful for
+     equi-recursive types).
+     However, I am not sure we need this; it'd be good to
+     write an example where this makes a difference.
+     I think that would be something like
+     nu x. { T = TNat; U = x.T -> x.T }:
+     mu (x: {T <: TNat; U <: x.T -> TNat}).
+     If the function type constructor is not contractive but only non-expansive,
+     typechecking this example needs to establish x.T <: TNat having in context
+     only x: {T <: TNat; U <: x.T -> TNat}.
+   *)
   Definition oForall τ1 τ2 := olty0
     (λI ρ v,
     (∃ t, ⌜ v = vabs t ⌝ ∧
      □ ∀ w, ▷ τ1 vnil ρ w → ▷ interp_expr τ2 (w .: ρ) t.|[w/])).
 
-  Lemma oTSel_pv w (l : label) args ρ v :
-    oTSel (pv w) l args ρ v ≡
-      (∃ ψ d, ⌜w.[ρ] @ l ↘ d⌝ ∧ d ↗n[ 0 ] ψ ∧ ▷ □ ψ vnil v)%I.
-  Proof. by rewrite /= path_wp_pv. Qed.
+  Definition oPrim b : olty Σ 0 := olty0 (λI ρ v, ⌜pure_interp_prim b v⌝).
 
-  Definition oPSing p : olty Σ 0 :=
-    olty0 (λI ρ v, ⌜alias_paths p.|[ρ] (pv v)⌝).
+  Class PersTyInterp (ty : Type) Σ :=
+    pers_ty_interp : ty → olty Σ 0.
+  Notation "p⟦ T ⟧" := (pers_ty_interp T%ty).
+  Global Arguments pers_ty_interp {_ _ _} !_ /.
+
+  Global Instance pinterp : PersTyInterp ty Σ :=
+    fix pinterp (T : ty) : olty Σ 0 :=
+    let _ := pinterp : PersTyInterp ty Σ in
+    match T with
+    | TTMem l L U => oTTMem l p⟦ L ⟧ p⟦ U ⟧
+    | TVMem l T' => oTVMem l p⟦ T' ⟧
+    | TAnd T1 T2 => oAnd p⟦ T1 ⟧ p⟦ T2 ⟧
+    | TOr T1 T2 => oOr p⟦ T1 ⟧ p⟦ T2 ⟧
+    | TLater T => oLater p⟦ T ⟧
+    | TPrim b => oPrim b
+    | TTop => oTop
+    | TBot => oBot
+    | TAll T1 T2 => oForall p⟦ T1 ⟧ p⟦ T2 ⟧
+    | TMu T => oMu p⟦ T ⟧
+    | TSel p l => oTSel p l
+    | TSing p => oPSing p
+    end.
+  (* Wrap this into ty_interp to reuse lemmas. *)
+  Global Instance pers_to_ty_interp : TyInterp ty Σ := flip pers_ty_interp vnil.
+  Global Arguments pers_to_ty_interp _ /.
+  Global Arguments ty_interp {_ _ _} _ /.
+
+  Global Instance interp_lemmas: TyInterpLemmas ty Σ.
+  Proof.
+    split => /=; induction T => sb1 sb2 w /=;
+      properness; rewrite ?scons_up_swap ?hsubst_comp; trivial; by f_equiv => ?.
+  Qed.
+
+  Global Instance interp_persistent T ρ v : Persistent (⟦ T ⟧ ρ v) := _.
+
+  Fixpoint def_interp_base (T : ty) : dlty Σ :=
+    match T with
+    | TTMem l L U => oDTMem l p⟦ L ⟧ p⟦ U ⟧
+    | TVMem l T' => oDVMem l p⟦ T' ⟧
+    | _ => Dlty "" (λI _ _, False)
+    end.
+
+  Global Instance def_interp_persistent T ρ d :
+    Persistent (dlty_car (def_interp_base T) ρ d).
+  Proof. destruct T; try apply _. Qed.
+
+  Implicit Types (l : label).
+
+  Definition def_interp T l := lift_dlty (def_interp_base T) l.
+
+  Definition defs_interp_and (interp1 interp2 : envPred dms Σ) : envPred dms Σ :=
+    λI ρ ds, interp1 ρ ds ∧ interp2 ρ ds.
+
+  Definition lift_dinterp_dms T : envPred dms Σ := λI ρ ds,
+    ∃ l d, ⌜ dms_lookup l ds = Some d ⌝ ∧ def_interp T l ρ d.
+
+  Fixpoint defs_interp T : envPred dms Σ :=
+    match T with
+    | TAnd T1 T2 => defs_interp_and (defs_interp T1) (defs_interp T2)
+    | TTop => λI ρ ds, True
+    | _ => lift_dinterp_dms T
+    end.
+
+  Global Instance defs_interp_persistent T ρ ds : Persistent (defs_interp T ρ ds).
+  Proof. induction T; try apply _. Qed.
+
+  (** Multi-definition typing *)
+  Definition idstp Γ T ds : iProp Σ :=
+    ⌜wf_ds ds⌝ ∧ □∀ ρ, ⌜path_includes (pv (ids 0)) ρ ds ⌝ → s⟦Γ⟧* ρ → defs_interp T ρ ds.|[ρ].
+  Global Arguments idstp /.
+
+  (* Fixpoint interp_env (Γ : ctx) (ρ : var → vl) : iProp Σ :=
+    match Γ with
+    | T :: Γ' => interp_env Γ' (stail ρ) ∧ ⟦ T ⟧ ρ (shead ρ)
+    | nil => True
+    end%I. *)
+
+  Notation "p⟦ Γ ⟧*" := (pers_ty_interp <$> Γ).
+  Notation "d⟦ T ⟧" := (def_interp_base T%ty).
+
+  Definition idtp  Γ T l d     := sdtp  p⟦Γ⟧* d⟦T⟧ l d.
+  (* Definition idstp Γ T ds      := sdstp p⟦Γ⟧* p⟦T⟧ ds. *)
+  Definition ietp  Γ T e       := setp  p⟦Γ⟧* p⟦T⟧ e.
+  Definition istpi Γ T1 T2 i j := sstpi p⟦Γ⟧* p⟦T1⟧ p⟦T2⟧ i j.
+  Definition iptp  Γ T p i     := sptp  p⟦Γ⟧* p⟦T⟧ p i.
+
+  Global Instance idtp_persistent Γ T l d: IntoPersistent' (idtp Γ T l d) | 0 := _.
+  Global Instance idstp_persistent Γ T ds: IntoPersistent' (idstp Γ T ds) | 0 := _.
+  Global Instance ietp_persistent Γ T e : IntoPersistent' (ietp Γ T e) | 0 := _.
+  Global Instance istpi_persistent Γ T1 T2 i j : IntoPersistent' (istpi Γ T1 T2 i j) | 0 := _.
+  Global Instance iptp_persistent Γ T p i : IntoPersistent' (iptp Γ T p i) | 0 := _.
+
+  Implicit Types (T : olty Σ 0) (TD : dlty Σ).
+
+  Local Notation IntoPersistent' P := (IntoPersistent false P P).
+  (* Avoid auto-dropping box (and unfolding) when introducing judgments persistently. *)
+  Global Instance sdtp_persistent Γ TD l d: IntoPersistent' (sdtp Γ TD l d) | 0 := _.
+  (* Global Instance sdstp_persistent Γ T ds: IntoPersistent' (sdstp Γ T ds) | 0 := _. *)
+  Global Instance setp_persistent Γ T e : IntoPersistent' (setp Γ T e) | 0 := _.
+  Global Instance sstpi_persistent Γ T1 T2 i j : IntoPersistent' (sstpi Γ T1 T2 i j) | 0 := _.
+  Global Instance sptp_persistent Γ T p i : IntoPersistent' (sptp Γ T p i) | 0 := _.
+
 End SemTypes.
+Notation "d ↗ ψ" := (dm_to_type 0 d ψ) (at level 20).
+Notation "p⟦ T ⟧" := (pers_ty_interp T%ty).
+Notation "p⟦ Γ ⟧*" := (pers_ty_interp <$> Γ).
+Notation "p⟦ T ⟧ₑ" := (interp_expr ⟦ T ⟧).
+(* Notation "⟦ T ⟧ₑ" := (interp_expr p⟦ T ⟧). *)
+(* Definition interp_env (Γ : ctx) : env -d> iPropO Σ := env_oltyped (pers_ty_interp <$> Γ).
+Global Arguments interp_env !_ _ /.
+Notation "⟦ Γ ⟧*" := (interp_env Γ). *)
+(* Notation "⟦ Γ ⟧*" := (env_oltyped (pers_ty_interp <$> Γ)). *)
+Notation "⟦ Γ ⟧*" := s⟦ p⟦ Γ ⟧* ⟧*.
+
+
+(** Single-definition typing *)
+Notation "Γ ⊨ {  l := d  } : T" := (idtp p⟦Γ⟧* p⟦T⟧ l d) (at level 74, d, l, T at next level).
+(** Multi-definition typing *)
+Notation "Γ ⊨ds ds : T" := (idstp p⟦Γ⟧* p⟦T⟧ ds) (at level 74, ds, T at next level).
+(** Expression typing *)
+Notation "Γ ⊨ e : T" := (ietp p⟦Γ⟧* p⟦T⟧ e) (at level 74, e, T at next level).
+Notation "Γ ⊨p p : T , i" := (iptp p⟦Γ⟧* p⟦T⟧ p i) (at level 74, p, T, i at next level).
+
+Notation "Γ ⊨ T1 , i <: T2 , j " := (istpi p⟦Γ⟧* p⟦T1⟧ p⟦T2⟧ i j) (at level 74, T1, T2, i, j at next level).
 
 Section SampleTypingLemmas.
   Context `{HdotG: dlangG Σ}.
